# baseURI: http://purl.org/dpn/dataset
# imports: http://www.w3.org/2003/01/geo/wgs84_pos
# imports: http://www.w3.org/2006/time
# imports: http://w3id.org/env/puv
# prefix: dpnd

@prefix dc: <http://purl.org/dc/terms/> .
@prefix dcterms: <http://purl.org/dc/terms/> .
@prefix j.0: <http://purl.org/dc/elements/1.1/> .
@prefix dpn: <http://purl.org/dpn/v0.8#> .
@prefix dpnd: <http://purl.org/dpn/dataset#> .
@prefix dpnd_old: <http://purl.org/dpn/dataset/v0.7.2> .
@prefix geo: <http://www.w3.org/2003/01/geo/wgs84_pos#> .
@prefix op: <http://environment.data.gov.au/def/op#> .
@prefix owl: <http://www.w3.org/2002/07/owl#> .
@prefix puv: <https://w3id.org/env/puv#> .
@prefix qudt: <http://qudt.org/schema/qudt/> .
@prefix rdf: <http://www.w3.org/1999/02/22-rdf-syntax-ns#> .
@prefix rdfs: <http://www.w3.org/2000/01/rdf-schema#> .
@prefix sosa: <http://www.w3.org/ns/sosa/> .
@prefix skos: <http://www.w3.org/2004/02/skos/core#> .
@prefix time: <http://www.w3.org/2006/time#> .
@prefix xml: <http://www.w3.org/XML/1998/namespace> .
@prefix xsd: <http://www.w3.org/2001/XMLSchema#> .

<http://purl.org/dpn/dataset>
  rdf:type owl:Ontology ;
  rdfs:comment "This ontology is being developed by CSIRO under the eReefs project for describing datasets, such as observational datasets. It imports the observable properties ontology which allows description of feature, substance or taxon, and quantity kinds." ;
  owl:imports dpn: ;
  owl:imports geo: ;
  owl:imports op: ;
  owl:imports puv: ;
  owl:imports qudt: ;
  owl:imports sosa: ;
  owl:imports time: ;
  owl:priorVersion <http://purl.org/dpn/dataset/v0.7.2> ;
  owl:versionIRI <http://purl.org/dpn/dataset/v0.8> ;
  owl:versionInfo "v0.8 eReefs Phase 5 2022" ;
  skos:changeNote "Additional alignment to OWL-Time added by SJDC - 2016-06-16" ;
  skos:changeNote "Incorporation of PUV-Ont added by ST - 2022-04 for eReefs Phase 5" ;
.

dpnd:BoundingBox
  rdf:type owl:Class ;
  rdfs:comment "A geospatial bounding box." ;
  rdfs:label "Bounding box" ;
  rdfs:subClassOf geo:SpatialThing ;
  rdfs:subClassOf [
      rdf:type owl:Restriction ;
      owl:onProperty dpnd:bbBottomRight ;
      owl:someValuesFrom geo:Point ;
    ] ;
  rdfs:subClassOf [
      rdf:type owl:Restriction ;
      owl:onProperty dpnd:bbTopLeft ;
      owl:someValuesFrom geo:Point ;
    ] ;
.
dpnd:Observation
  rdf:type owl:Class ;
  rdfs:comment "A dataset which contains information about related observations of a single property. These may be directly observed (field observations) or modelled" ;
  rdfs:label "Observation" ;
  rdfs:subClassOf dpn:Dataset ;
  rdfs:subClassOf puv:Parameter ;
  rdfs:subClassOf [
    rdf:type owl:Restriction ;
    owl:onProperty puv:parameter ;
    owl:someValuesFrom puv:Parameter ;
  ] ;
  rdfs:subClassOf [
      rdf:type owl:Restriction ;
      owl:onProperty dpnd:spatial ;
      owl:someValuesFrom geo:SpatialThing ;
    ] ;
  rdfs:subClassOf [
      rdf:type owl:Restriction ;
      owl:onProperty dpnd:temporal ;
      owl:someValuesFrom dpnd:TimeInterval ;
    ] ;
.
dpnd:TimeInterval
  rdf:type owl:Class ;
  rdfs:label "Time interval" ;
  rdfs:subClassOf dc:PeriodOfTime ;
  rdfs:subClassOf time:Interval ;
.
dpnd:bbBottomRight
  rdf:type owl:ObjectProperty ;
  rdfs:comment "Bottom-right (South-East-Nadir) coordinate of a geographical bounding box" ;
  rdfs:domain dpnd:BoundingBox ;
  rdfs:label "bbBottomRight" ;
  rdfs:range geo:Point ;
.
dpnd:bbTopLeft
  rdf:type owl:ObjectProperty ;
  rdfs:comment "Top-left (North-West-Zenith) coordinate of a geographical bounding box" ;
  rdfs:domain dpnd:BoundingBox ;
  rdfs:label "bbTopLeft" ;
  rdfs:range geo:Point ;
.
dpnd:end
  rdf:type owl:DatatypeProperty ;
  rdfs:comment "The end of a time interval" ;
  rdfs:domain dpnd:TimeInterval ;
  rdfs:label "end" ;
  rdfs:range xsd:dateTime ;
.
dpnd:relatedFeature
  rdf:type owl:ObjectProperty ;
  rdfs:comment "related feature of interest" ;
  rdfs:label "related feature" ;
.
dpnd:relatedQuantityKind
  rdf:type owl:ObjectProperty ;
  rdfs:comment "related quantity kind" ;
  rdfs:label "related quantity kind" ;
.
dpnd:relatedSubstanceOrTaxon
  rdf:type owl:ObjectProperty ;
  rdfs:label "related substance or taxon" ;
.
dpnd:spatial
  owl:equivalentProperty dc:spatial ;
  rdf:type owl:ObjectProperty ;
  rdfs:comment "The spatial location (e.g. point or bounding box) where observations were made" ;
  rdfs:domain dpnd:Observation ;
  rdfs:label "spatial" ;
  rdfs:range geo:SpatialThing ;
.
dpnd:start
  rdf:type owl:DatatypeProperty ;
  rdfs:comment "The beginning of a time-range" ;
  rdfs:domain dpnd:TimeInterval ;
  rdfs:label "start" ;
  rdfs:range xsd:dateTime ;
.
dpnd:temporal
  rdf:type owl:ObjectProperty ;
  rdfs:comment "The time-range for which observations were made" ;
  rdfs:domain dpnd:Observation ;
  rdfs:label "temporal" ;
  rdfs:range dpnd:TimeInterval ;
.
#----------------------------------------------------------------------
# PUV-ont redefinitions because the IRI doesn't seem to parse properly
# Source: https://github.com/CSIRO-enviro-informatics/PUV-ont/blob/main/rdf/puv.ttl
#----------------------------------------------------------------------
puv:BiologicalEntity
  rdf:type owl:Class ;
  rdfs:comment """NVS Biological entity (S25) Terms used to describe biological entities (organisms or parts thereof) in the BODC Parameter Usage Vocabulary.

  See: http://vocab.nerc.ac.uk/collection/S25/

  Also see: Related NVS Vocabs S09 (size), S10 (gender), S11 (stage), S12 (sub-component), S13 (sub-group), S14 (shape), S15 (colour)""" ;
  rdfs:label "Biological entity (S25)" ;
  rdfs:seeAlso <http://vocab.nerc.ac.uk/collection/S25/> ;
  rdfs:subClassOf skos:Concept ;
  rdfs:subClassOf puv:Entity ;
.
puv:ChemicalEntity
  rdf:type owl:Class ;
  rdfs:comment """NVS Chemical substance (S27) terms for chemicals whose quantity in a matrix is determined to generate measurements in the BODC parameter usage vocabulary semantic model.
  Includes elements, compounds, isotopes and mixtures.

  See: http://vocab.nerc.ac.uk/collection/S27/
  """ ;
  rdfs:label "ChemicalEntity (S27)" ;
  rdfs:seeAlso <http://vocab.nerc.ac.uk/collection/S27/> ;
  rdfs:subClassOf skos:Concept ;
  rdfs:subClassOf puv:Entity ;
.
puv:Matrix
  owl:equivalentClass dpnd_old:Medium ;
  rdf:type owl:Class ;
  rdfs:comment """NVS Matrix (S26) terms used to describe the medium in which a measurement was made in the semantic model that underpins the BODC parameter discovery vocabulary.

  See: https://vocab.nerc.ac.uk/collection/S26/

  Also see: Related NVS Vocabs S21 (sphere), S22 (sphere sub-group), S23 (phase), S24 (phase sub-group)
  """ ;
  rdfs:label "Matrix (S26)" ;
  rdfs:seeAlso <https://vocab.nerc.ac.uk/collection/S26/> ;
  rdfs:subClassOf skos:Concept ;
  rdfs:subClassOf [
      rdf:type owl:Restriction ;
      owl:allValuesFrom puv:MatrixComponent ;
      owl:onProperty puv:isComposedOf ;
    ] ;
.
puv:matrix
  owl:equivalentProperty dpnd_old:relatedMedium ;
  owl:equivalentProperty op:matrix ;
  rdf:type owl:ObjectProperty ;
  rdfs:comment """The context / container / medium within which the property of an entity is observed.
  Reference to the NVS Matrix (S26) term for this matrix of this observation.
  This property on a dpn:Observation resource, this overrides the equivalent property value inherited from dpn:Observation -> parameter.
  """ ;
  rdfs:domain puv:Parameter ;
  rdfs:label "matrix" ;
  rdfs:range puv:Matrix ;
.
puv:MMRel
  rdf:type owl:Class ;
  rdfs:comment "NVS Measurement-matrix relationship (S02) terms used to describe the relationship between the 'where theme' and the 'what theme' in the BODC semantic model for measured phenomena descriptions" ;
  rdfs:label "MMRel (S02)" ;
  rdfs:seeAlso <https://vocab.nerc.ac.uk/collection/S02/> ;
  rdfs:subClassOf skos:Concept ;
.
puv:matrixRelationship
  owl:equivalentProperty puv:matrixRelationship ;
  rdf:type owl:ObjectProperty ;
  rdfs:comment """Reference to the NVS Measurement-matrix relationship (S02) term for this observation.
  This property on a dpn:Observation resource, this overrides the equivalent property value inherited from dpn:Observation -> parameter.
  """ ;
  rdfs:domain puv:Parameter ;
  rdfs:label "matrixRelationship" ;
  rdfs:range puv:MMRel ;
.
puv:Method
  rdf:type owl:Class ;
  rdfs:comment "NVS Data Processing Method (S05) or AnalyticalMethod (S04) or Sample Preparation method (S03) used to make the observation" ;
  rdfs:label "Method (NVS S03 or S04 or S05)" ;
.
puv:method
  owl:equivalentProperty op:procedure
  rdf:type owl:ObjectProperty ;
  rdfs:comment """The procedure or sensor system used in making the observation or estimate of property value.
  Reference to the NVS Method (S03 or S04 or S05) which is the object of interest.
  This property on a dpn:Observation resource, this overrides the equivalent property value inherited from dpn:Observation -> parameter.
  """ ;
  rdfs:label "method" ;
  rdfs:range puv:Method ;
.
puv:Entity
  owl:equivalentClass op:SubstanceOrTaxon ;
  owl:equivalentClass op:Substance ;
  owl:equivalentClass op:Taxon ;
  rdf:type owl:Class ;
  rdfs:comment "NVS BiologicalEntity (S25) or ChemicalEntity (S27) or PhysicalEntity (S29) being observed." ;
  rdfs:label "Entity (NVS S25 or S27 or S29)" ;
.
puv:objectOfInterest
  owl:equivalentProperty dpnd_old:relatedFeature ;
  owl:equivalentProperty dpnd_old:relatedSubstanceOrTaxon ;
  owl:equivalentProperty op:featureOfInterest ;
  owl:equivalentProperty op:objectOfInterest ;
  owl:equivalentProperty puv:biologicalObject ;
  owl:equivalentProperty puv:chemicalObject ;
  owl:equivalentProperty puv:physicalObject ;
  owl:equivalentProperty qudt:generalization ;
  rdf:type owl:ObjectProperty ;
  rdfs:comment "NVS Entity which is the object of interest for these observations. Can be a chemical, biological, or physical entity." ;
  rdfs:domain puv:Parameter ;
  rdfs:label "objectOfInterest" ;
  rdfs:range puv:Entity ;
.
puv:PhysicalEntity
  rdfs:type owl:Class ;
  rdfs:comment """NVS Physical Entity (S29) terms used to describe physical entities in the BODC Parameter Usage Vocabulary.

  See http://vocab.nerc.ac.uk/collection/S29/

  Also see related NVS Vocabularies: S18 (name), S19 (sub-group), S20 (datum)
  """ ;
  rdfs:label "PhysicalEntity (NVS S29)" ;
  rdfs:seeAlso <http://vocab.nerc.ac.uk/collection/S29/> ;
  rdfs:subClassOf skos:Concept ;
  rdfs:subClassOf puv:Entity ;
.
puv:Property
  owl:equivalentClass op:QualityKind ;
  owl:equivalentClass op:ScaledQuantityKind ;
  owl:equivalentClass qudt:QuantityKind;
  rdf:type owl:Class ;
  rdfs:comment "NVS Property (S06) terms that may be used to specify the property element of a parameter (part of the 'what' theme) in the BODC parameter semantic model" ;
  rdfs:label "Property (NVS S06)" ;
  rdfs:seeAlso <https://vocab.nerc.ac.uk/collection/S06/> ;
  rdfs:subClassOf skos:Concept ;
  rdfs:subClassOf sosa:ObservableProperty ;
.
puv:property
  owl:equivalentProperty dpnd_old:relatedQuantityKind ;
  owl:equivalentProperty qudt:hasQuantityKind ;
  rdf:type owl:ObjectProperty ;
  rdfs:comment """Reference to the NVS S06 property or attribute that is being measured, which must be associated with either an object of interest or a matrix or both
  This property on a dpn:Observation resource, this overrides the equivalent property value inherited from dpn:Observation -> parameter.
  """ ;
  rdfs:domain puv:Parameter ;
  rdfs:label "property" ;
  rdfs:range puv:Property ;
.
puv:ParameterStatistic
  rdf:type owl:Class ;
  rdfs:comment "NVS Parameter Statistic (S07)  terms that may be used for a parameter statistic (part of the what theme) in the BODC parameter semantic model" ;
  rdfs:label "ParameterStatistic (NVS S07)" ;
  rdfs:seeAlso <https://vocab.nerc.ac.uk/collection/S07/> ;
  rdfs:subClassOf skos:Concept ;
.
puv:statistic
  rdf:type owl:ObjectProperty ;
  rdfs:comment """Reference to the NVS S07 term that describes the statistical treatment of the observation.
  This property on a dpn:Observation resource, this overrides the equivalent property value inherited from dpn:Observation -> parameter.
  """ ;
  rdfs:domain puv:Parameter ;
  rdfs:label "statistic" ;
  rdfs:range puv:ParameterStatistic ;
.
puv:UnitOfMeasurement
  owl:equivalentClass qudt:Unit ;
  rdf:type owl:Class ;
  rdfs:comment "NVS Unit of Measurement (P06) terms approved for use by BODC to describe the measurement units for data held in its repositories." ;
  rdfs:label "UnitOfMeasurement (NVS P06)" ;
  rdfs:seeAlso <https://vocab.nerc.ac.uk/collection/P06/> ;
  rdfs:subClassOf skos:Concept ;
.
puv:uom
  owl:equivalentProperty qudt:unit ;
  rdf:type owl:ObjectProperty ;
  rdfs:comment """Reference to the NVS P06 term that specifies the scale or unit of measurement for the observation.
  This property on a dpn:Observation resource, this overrides the equivalent property value inherited from dpn:Observation -> parameter.

  If no suitable puv:Unit exists, then use qudt:unit (targetting a qudt:Unit resource) instead.
  """ ;
  rdfs:label "uom" ;
  rdfs:range puv:UnitOfMeasurement ;
.

puv:Parameter
  owl:equivalentClass op:PropertyKind ;
  owl:equivalentClass sosa:ObservableProperty ;
  owl:equivalentClass sosa:FeatureOfInterest ;
  rdf:type owl:Class ;
  rdfs:comment "Terms built using the BODC parameter semantic model designed to describe individual measured phenomena. May be used to mark up sets of data such as a NetCDF array or spreadsheet column" ;
  rdfs:comment "Scientific variable in databases and data files" ;
  rdfs:label "Parameter (NVS P01)" ;
  rdfs:seeAlso <https://vocab.nerc.ac.uk/collection/P01/> ;
  rdfs:subClassOf skos:Concept ;
.
puv:parameter
  owl:equivalentProperty op:property ;
  owl:equivalentProperty sosa:observedProperty ;
  rdf:type owl:ObjectProperty ;
  rdfs:comment "The NVS P01 Parameter that this Observation should inherit other NVS-related properties from. These properties can then be overridden if necessary." ;
  rdfs:domain dpnd:Observation ;
  rdfs:label "parameter" ;
  rdfs:range puv:Parameter ;
  rdfs:seeAlso <https://vocab.nerc.ac.uk/collection/P01/> ;
.
